benchmarks/lean/dafnybench/poor/unformatted/dafny-duck_tmp_tmplawbgxjo_p1_SumArray.lean
@@ -18,11 +18,11 @@ Recursively computes the sum of elements in an array.
 Given an array of integers, returns their sum.
 Example:  -> 9
 -/
-partial def Sum (xs : Array Int) : Int :=
+partial def Sum_ (xs : Array Int) : Int :=
 if xs.size = 0 then
 0
 else
-Sum (xs.extract 0 (xs.size - 1)) + xs[xs.size - 1]!
+Sum_ (xs.extract 0 (xs.size - 1)) + xs[xs.size - 1]!
 
 /--
 Takes an array of integers and returns their sum.
@@ -34,4 +34,4 @@ def SumArray (xs : Array Int) : Int := sorry
 Specification for SumArray ensuring it returns the correct sum
 -/
 theorem SumArray_spec (xs : Array Int) (s : Int) :
-s = SumArray xs → s = Sum xs := sorry
+s = SumArray xs → s = Sum_ xs := sorry
